Adding boiler plate code that links SplinterTree lemmas with BranchTree lemmas

Splinter/BranchTreeInterp.i.dfy
@@ -133,46 +133,102 @@ module BranchTreeInterpMod {
       }
     }
 
-    predicate ValidLookupForBranchEquivalent(cache0: CacheIfc.Variables,
-                                             cache1: CacheIfc.Variables,
-                                             receipt0: BranchReceipt,
-                                             receipt1: BranchReceipt)
-    {
-      && var lookup0 := receipt0.branchPath;
-      && var lookup1 := receipt1.branchPath;
-      && lookup0.key == lookup1.key
-      && lookup0.Valid(cache0)
-      && lookup1.Valid(cache1)
-    }
-
-    predicate RootEquivalentForBranchReceipts(cache0: CacheIfc.Variables,
-                                              cache1: CacheIfc.Variables,
-                                              receipt0: BranchReceipt,
-                                              receipt1: BranchReceipt)
-    {
-      && receipt0.Valid(cache0)
-      && receipt1.Valid(cache1)
-      && var cu0 := receipt0.branchTree.Root();
-      && var cu1 := receipt1.branchTree.Root();
-      && cu0 == cu1
-      && CacheIfc.ReadValue(cache0, cu0) == CacheIfc.ReadValue(cache1, cu1)
-    }
-
-    lemma BranchLookupsEquivalent(v: Variables,
+    lemma BranchLookupsEquivalent(v: SplinterTreeMachineMod.Variables,
                                   cache0: CacheIfc.Variables,
                                   cache1: CacheIfc.Variables,
                                   receipt0: BranchReceipt,
                                   receipt1: BranchReceipt)
 
-      requires ValidLookupForBranchEquivalent(cache0, cache1, receipt0, receipt1)
-      requires RootEquivalentForBranchReceipts(cache0, cache1, receipt0, receipt1)
-      requires DiskViewsEquivalent(cache0.dv, cache1.dv, IReadsLookup(cache0, receipt0.branchPath))
-      ensures  receipt0 == receipt1
-      {
+        requires ValidLookupForBranchEquivalent(cache0, cache1, receipt0, receipt1)
+        requires RootEquivalentForBranchReceipt(cache0, cache1, receipt0, receipt1)
+        requires DiskViewsEquivalent(cache0.dv, cache1.dv, IReadsLookup(cache0, receipt0.branchPath))
+        ensures  receipt0 == receipt1
+     {
         var lookup0 := receipt0.branchPath;
         var lookup1 := receipt1.branchPath;
         var minLookup := min(|lookup0.steps|, |lookup1.steps|);
         BranchLookupsEquivalentInductive(v, cache0, cache1, lookup0, lookup1, minLookup);
       }
+
+
+   predicate BranchLookupEquivalentRequirements(v: SplinterTreeMachineMod.Variables,
+                                    cache0: CacheIfc.Variables,
+                                    cache1: CacheIfc.Variables,
+                                    receipts0: seq<BranchReceipt>,
+                                    receipts1: seq<BranchReceipt>)
+   {
+     && forall i | 0 <= i < min(|receipts0|, |receipts1|) :: ValidLookupForBranchEquivalent(cache0, cache1, receipts0[i], receipts1[i])
+     && forall i | 0 <= i < min(|receipts0|, |receipts1|) :: DiskViewsEquivalent(cache0.dv, cache1.dv, IReadsLookup(cache0, receipts0[i].branchPath))
+   }
+
+   predicate ValidLookupForBranchEquivalent(cache0: CacheIfc.Variables,
+                                            cache1: CacheIfc.Variables,
+                                            receipt0: BranchReceipt,
+                                            receipt1: BranchReceipt)
+   {
+     && var lookup0 := receipt0.branchPath;
+     && var lookup1 := receipt1.branchPath;
+     && lookup0.key == lookup1.key
+     && lookup0.Valid(cache0)
+     && lookup1.Valid(cache1)
+   }
+
+   predicate RootEquivalentForBranchReceipt(cache0: CacheIfc.Variables,
+                                             cache1: CacheIfc.Variables,
+                                             receipt0: BranchReceipt,
+                                             receipt1: BranchReceipt)
+   {
+     && receipt0.Valid(cache0)
+     && receipt1.Valid(cache1)
+     && var cu0 := receipt0.branchTree.Root();
+     && var cu1 := receipt1.branchTree.Root();
+     && cu0 == cu1
+     && CacheIfc.ReadValue(cache0, cu0) == CacheIfc.ReadValue(cache1, cu1)
+   }
+
+   lemma RootEquivalentForBranchReceipts(v: SplinterTreeMachineMod.Variables,
+                                    cache0: CacheIfc.Variables,
+                                    cache1: CacheIfc.Variables,
+                                    receipts0: seq<BranchReceipt>,
+                                    receipts1: seq<BranchReceipt>)
+      requires BranchLookupEquivalentRequirements(v, cache0, cache1, receipts0, receipts1)
+      ensures forall i | 0 <= i < min(|receipts0|,|receipts1|) :: RootEquivalentForBranchReceipt(cache0, cache1, receipts0[i], receipts1[i])
+      ensures |receipts0| == |receipts1|
+   {
+
+   }
+
+   lemma BranchReceiptsEquivalentInductive(v: SplinterTreeMachineMod.Variables,
+                                    cache0: CacheIfc.Variables,
+                                    cache1: CacheIfc.Variables,
+                                    receipts0: seq<BranchReceipt>,
+                                    receipts1: seq<BranchReceipt>,
+                                    count: nat)
+      requires BranchLookupEquivalentRequirements(v, cache0, cache1, receipts0, receipts1)
+      ensures forall i | 0 <= i < count :: receipts0[i] == receipts1[i]
+      ensures |receipts0| == |receipts1|
+    {
+      if (0 < count) {
+        BranchReceiptsEquivalentInductive(v, cache0, cahe1, receipts0, receipts1, count-1);
+        BranchLookupsEquivalent(v, cache0, cache1, receipts0[count-1], receipts1[count-1]);
+      }
+    }
+
+    lemma BranchReceiptsEquivalent(v: SplinterTreeMachineMod.Variables,
+                                  cache0: CacheIfc.Variables,
+                                  cache1: CacheIfc.Variables,
+                                  receipts0: seq<BranchReceipt>,
+                                  receipts1: seq<BranchReceipt>)
+
+
+      requires BranchLookupEquivalentRequirements(v, cache0, cache1, receipts0, receipts1)
+      requires forall i | 0 <= i < min(|receipts0|, |receipts1|) :: RootEquivalentForBranchReceipt(cache0, cache1, receipts0[i], receipts1[i])
+      ensures forall i | 0 <= i < min(|receipts0|, |receipts1|) :: receipts0[i] == receipts1[i]
+      ensures |receipts0| == |receipts1|
+    {
+
+      var count := min(|receipts0|, |receipts1|);
+      BranchReceiptsEquivalentInductive(v, cache0, cache1, receipts0, receipts1, count);
+    }
 
 }
